Source/Dafny/Compilers/Compiler-go.cs
@@ -1002,6 +1002,11 @@ namespace Microsoft.Dafny {
       public ConcreteSyntaxTree/*?*/ CreateMethod(Method m, List<TypeArgumentInstantiation> typeArgs, bool createBody, bool forBodyInheritance, bool lookasideBody) {
         return Compiler.CreateMethod(m, typeArgs, createBody, ClassName, AbstractMethodWriter, ConcreteMethodWriter, forBodyInheritance, lookasideBody);
       }
+
+      public ConcreteSyntaxTree CreateMockMethod(Method m) {
+        throw new NotImplementedException();
+      }
+
       public ConcreteSyntaxTree/*?*/ CreateFunction(string name, List<TypeArgumentInstantiation> typeArgs, List<Formal> formals, Type resultType, Bpl.IToken tok, bool isStatic, bool createBody, MemberDecl member, bool forBodyInheritance, bool lookasideBody) {
         return Compiler.CreateFunction(name, typeArgs, formals, resultType, tok, isStatic, createBody, member, ClassName, AbstractMethodWriter, ConcreteMethodWriter, forBodyInheritance, lookasideBody);
       }
