Source/Dafny/Compilers/Compiler.cs
@@ -93,6 +93,7 @@ namespace Microsoft.Dafny {
     protected abstract string GetHelperModuleName();
     protected interface IClassWriter {
       ConcreteSyntaxTree/*?*/ CreateMethod(Method m, List<TypeArgumentInstantiation> typeArgs, bool createBody, bool forBodyInheritance, bool lookasideBody);
+      ConcreteSyntaxTree/*?*/ CreateMockMethod(Method m);
       ConcreteSyntaxTree/*?*/ CreateFunction(string name, List<TypeArgumentInstantiation> typeArgs, List<Formal> formals, Type resultType, Bpl.IToken tok, bool isStatic, bool createBody,
         MemberDecl member, bool forBodyInheritance, bool lookasideBody);
       ConcreteSyntaxTree/*?*/ CreateGetter(string name, TopLevelDecl enclosingDecl, Type resultType, Bpl.IToken tok, bool isStatic, bool isConst, bool createBody, MemberDecl/*?*/ member, bool forBodyInheritance);  // returns null iff !createBody
@@ -1255,6 +1256,11 @@ namespace Microsoft.Dafny {
       public ConcreteSyntaxTree/*?*/ CreateMethod(Method m, List<TypeArgumentInstantiation> typeArgs, bool createBody, bool forBodyInheritance, bool lookasideBody) {
         return createBody ? block : null;
       }
+
+      public ConcreteSyntaxTree CreateMockMethod(Method m) {
+        throw new NotImplementedException();
+      }
+
       public ConcreteSyntaxTree/*?*/ CreateFunction(string name, List<TypeArgumentInstantiation> typeArgs, List<Formal> formals, Type resultType, Bpl.IToken tok, bool isStatic, bool createBody, MemberDecl member, bool forBodyInheritance, bool lookasideBody) {
         return createBody ? block : null;
       }
@@ -1766,8 +1772,14 @@ namespace Microsoft.Dafny {
           if (m.Body == null && !(c is TraitDecl && !m.IsStatic) &&
               !(!DafnyOptions.O.DisallowExterns && (Attributes.Contains(m.Attributes, "dllimport") || (IncludeExternMembers && Attributes.Contains(m.Attributes, "extern"))))) {
             // A (ghost or non-ghost) method must always have a body, except if it's an instance method in a trait.
-            if (Attributes.Contains(m.Attributes, "axiom") || (!DafnyOptions.O.DisallowExterns && Attributes.Contains(m.Attributes, "extern"))) {
+            if (Attributes.Contains(m.Attributes, "axiom")) {
               // suppress error message
+            } else if (!DafnyOptions.O.DisallowExterns && Attributes.Contains(m.Attributes, "extern")) {
+              if (Attributes.Contains(m.Attributes, "mock") && m.IsStatic &&
+                  m.Ins.Count == 0 && m.Outs.Count == 1 &&
+                  m.Ens.Count == 1 && m.Ens.Any(ensure => ensure.E is FreshExpr)) {
+                classWriter.CreateMockMethod(m);
+              }
             } else {
               Error(m.tok, "Method {0} has no body", errorWr, m.FullName);
             }
